WIP on memory

RMemory.v
@@ -90,6 +90,69 @@ Section MemoryInd.
 
 End MemoryInd.
 
+Inductive equal_memory {V: Type} : memory V -> memory V -> Prop :=
+  equal_memory_intro:
+    forall m m',
+      Env.Equal (values m) (values m') ->
+      Env.Equiv equal_memory (instances m) (instances m') ->
+      equal_memory m m'.
+Infix "≋" := equal_memory (at level 70, no associativity).
+
+Lemma equal_memory_refl:
+  forall {V} (m: memory V),
+    m ≋ m.
+Proof.
+  induction m as [? IH] using memory_ind'.
+  constructor.
+  - reflexivity.
+  - split.
+    + reflexivity.
+    + intros ** Find ?.
+      eapply Env.Props.P.F.MapsTo_fun in Find; eauto.
+      rewrite <-Find; eauto.
+Qed.
+
+Lemma equal_memory_sym:
+  forall {V} (m m': memory V),
+    m ≋ m' -> m' ≋ m.
+Proof.
+  induction m as [? IH] using memory_ind'.
+  inversion_clear 1 as [?? Vals Insts].
+  constructor.
+  - now symmetry.
+  - split; destruct Insts as (? & HMapsTo).
+    + now symmetry.
+    + intros ** Find ?.
+      eapply HMapsTo in Find; eauto.
+Qed.
+
+Lemma equal_memory_trans:
+  forall {V} (m1 m2 m3: memory V),
+    m1 ≋ m2 -> m2 ≋ m3 -> m1 ≋ m3.
+Proof.
+  induction m1 as [? IH] using memory_ind'.
+  inversion_clear 1 as [?? Vals12 Insts12];
+    inversion_clear 1 as [?? Vals23 Insts23].
+  constructor.
+  - now rewrite Vals12.
+  - split; destruct Insts12 as (In12 & HMapsTo12), Insts23 as (?& HMapsTo23).
+    + now setoid_rewrite In12.
+    + intros ** Find1 Find3.
+      assert (exists e'', Env.MapsTo k e'' (instances m2)) as (e'' &?).
+      { setoid_rewrite Env.Props.P.F.find_mapsto_iff.
+        rewrite <-Env.In_find, <-In12, Env.In_find.
+        setoid_rewrite <-Env.Props.P.F.find_mapsto_iff; eauto.
+      }
+      pose proof Find1.
+      apply (HMapsTo12 _ _ e'') in Find1; auto.
+      apply (HMapsTo23 _ e'') in Find3; eauto.
+Qed.
+
+Add Parametric Relation V : (memory V) (equal_memory)
+    reflexivity proved by (@equal_memory_refl V)
+    symmetry proved by (@equal_memory_sym V)
+    transitivity proved by (@equal_memory_trans V)
+      as equal_memory_rel.
 
 (** ** Properties *)
 
